	Let us consider $\frac{\vec{z}_1 + \vec{z}_1 + 1}{\vec{z}_1-\vec{z}_2+1}$, then
	\begin{align}
		\vec{z}_1 + \vec{z}_1 + 1 &= \myvec{2 \\ -1} + \myvec{ 2 \\ -1} + \myvec{ 1 \\ 0} \\
		&= \myvec{5 \\ -2}\\
		\vec{z}_1 - \vec{z}_2 + 1 &= \myvec{2 \\ -1} - \myvec{ 1 \\ 1} + \myvec{ 1 \\ 0} \\
		&= \myvec{2 \\ -2} \\ 
		\frac{\vec{z}_1 + \vec{z}_1 + 1}{\vec{z}_1-\vec{z}_2+1} &= \frac{\myvec{5 \\ -2}}{\myvec{2 \\ -2}}\label{eq:sol_comp_12result} 
	\end{align}
	The modulus of a complex number $\myvec{a \\ b}$ is defined as $\sqrt{a^{2} + b^{2}}$.
	Therefore, 
	\begin{align}
		\norm{\vec{z}_1 + \vec{z}_1 + 1} &= \sqrt{5^{2} + (-2)^{2}} \\ 
		&= \sqrt{29}  \label{eq:sol_comp_12res_1} \\
		\norm{\vec{z}_1 -  \vec{z}_2 + 1} &= \sqrt{2^{2} + (-2)^{2}} \\ 
		&= \sqrt{8} \label{eq:sol_comp_12res_2}
	\end{align}
Putting together \eqref{eq:sol_comp_12res_1} and \eqref{eq:sol_comp_12res_2}, we have
\begin{align}
		\norm{\frac{\vec{z}_1 + \vec{z}_1 + 1}{\vec{z}_1-\vec{z}_2+1}}	 = \frac{\sqrt{29}}{\sqrt{8}}
\end{align}
