
We have, $$\vec{u}= \myvec{1 \\ 3 \\ 7},\vec{v}= \myvec{7 \\ -1 \\ 8}$$
\begin{align}
 \vec{p}=\left[\frac{\myvec{1 \\ 3 \\ 7}^T\myvec{7 \\ -1 \\ 8}}{{\norm{\begin{matrix}7 \\ -1 \\ 8\end{matrix}}}^2}\right] \myvec{7 \\ -1 \\ 8}\\
\vec{p}=\left[\frac{(7-3+56)}{\left(\sqrt{7^2+(-1)^2+8^2}\right)^2}\right]\myvec{7 \\ -1 \\ 8}\\
\vec{p}=\frac{13}{25} \myvec{7 \\ -1 \\ 8}= \myvec{\frac{92}{25} \\[0.2cm] -\frac{13}{25} \\[0.2cm] \frac{21}{5}}
\end{align}

Hence the projection of $\vec{u}$ on $\vec{v}$ is $$\vec{p}=\myvec{\frac{92}{25} \\[0.2cm] -\frac{13}{25} \\[0.2cm] \frac{21}{5}}$$


