The direction vectors of $\vec{A}-\vec{B}$, $\vec{A}-\vec{C}$ and $\vec{B}-\vec{C}$ are
\begin{align}
	\vec{A}-\vec{B} =\myvec{-1 \\ 1} \\
	\vec{A}-\vec{C} =\myvec{-5 \\ -5}\\
	\vec{B}-\vec{C} =\myvec{-4 \\ -6} 
\end{align}
\begin{enumerate}
\item \begin{align} {(\vec{A}-\vec{B})}^T  (\vec{B}-\vec{C})  =   \myvec{ -1 \\ 1 }  \myvec{ -4 \\ -6 } = -2 \end{align}
\begin{align}{(\vec{A}-\vec{B})}^T  (\vec{B}-\vec{C}) = -2 \neq 0 \end{align}
Sides $\vec{A}-\vec{B}$ and $\vec{B}-\vec{C}$ of triangle are not perpendicular.

\item \begin{align}{(\vec{A}-\vec{C})}^T  (\vec{B}-\vec{C}) =  \myvec{ -5 \\ -5 }  \myvec{ -4 \\ -6 } = 50\end{align}
\begin {align}{(\vec{A}-\vec{C})}^T  (\vec{B}-\vec{C}) = 50 \neq 0 \end {align}
Sides $\vec{A}-\vec{C}$ and $\vec{B}-\vec{C}$ of triangle are not perpendicular.

\item \begin{align}{(\vec{A}-\vec{B})}^T  (\vec{A}-\vec{C}) =  \myvec{ -1 \\ 1 }  \myvec{ -5 \\ -5 } = 0\end{align}
\begin {align}{(\vec{A}-\vec{B})}^T  (\vec{A}-\vec{C}) = 0  \end {align}
Sides $\vec{A}-\vec{B}$ and  $\vec{A}-\vec{C}$  of triangle are perpendicular to each other and the right angle at vertex \myvec{ 4 \\ 4 }, and the following figure represents the triangle formed by given points $\vec{A}$, $\vec{B}$ and $\vec{C}$.  
\end{enumerate}
