\begin{equation}
\vec{a^Tb}=\myvec{3&-4&5} \myvec{-2\\1\\-3}  
\end{equation}
\begin{equation}
=(3\times -2)+(-4\times 1)+(5\times -3)
\end{equation}
\begin{equation}
=-25    
\end{equation}

\begin{equation}
\vec{a \times b} &= \myvec{0 & 5 & -4\\ 5 & 0 & -3\\ -(-4) & 3 &  0} \myvec{-2\\1\\3}    
\end{equation}
\\
\begin{equation}
\vec{a \times b}  =  \myvec{(0 \times -2)  +  (-5 \times 1)  +  (-4 \times -3)\\(5 \times -2)  +  (0 \times 1)  +  (-3 \times -3)\\(4 \times -2)  +  (3 \times 1)  + (0 \times -3)}    
\end{equation}
\\
\begin{equation}
\vec{a \times b}  =  \myvec{7\\-1\\5}    
\end{equation}
