\renewcommand{\theequation}{\theenumi}
\begin{enumerate}[label=\thesubsection.\arabic*.,ref=\thesubsection.\theenumi]
\numberwithin{equation}{enumi}
\item {\em Definition: }Let $\vec{x} \in \mathbb{R}^2, f\brak{\vec{x}} \in \mathbb{R}$.  Then, 
\begin{align}
\frac{df\brak{\vec{x}}}{d\vec{x}} = \myvec{\frac{\partial f(\vec{x})}{\partial x_1}\\\frac{\partial f(\vec{x})}{\partial x_2}}
\end{align}
\item 
\begin{align}
\begin{split}
\frac{d\vec{x}}{dx_1} &= \myvec{\frac{dx_1}{dx_1} \\ \frac{dx_1}{dx_1}} 
\\
&= \myvec{1\\m} = \vec{m}
\end{split}
\label{eq:calc_m_diff}
\end{align}
\item Show that 
\begin{align}
\begin{split}
\frac{d\brak{\vec{u}^T\vec{x}}}{d\vec{x}} &= \vec{u}
\\
\frac{d\brak{\vec{x}^T\vec{V}\vec{x}}}{d\vec{x}} &= 2\vec{V}^T\vec{x}
\end{split}
\label{eq:calc_vec_diff}
\end{align}
\item Differentiating \eqref{eq:conic_quad_form}
%\eqref{eq:ellipse_vec}  
with respect to $x_1$,
%
%\numberwithin{equation}{enumi}
\begin{align}
\label{eq:ellipse_tangent_der}
\sbrak{\frac{d\brak{\vec{x}^T\vec{V}\vec{x}}}{d\vec{x}}}^T\frac{d\vec{x}}{dx_1}
+2\frac{d\brak{\vec{u}^T\vec{x}}}{\vec{x}} \frac{d\vec{x}}{dx_1}
= 0
\\
\implies 2\brak{\vec{V}^T\vec{x}+\vec{u}}\vec{m}  = 0  
\end{align}
from \eqref{eq:calc_m_diff} and \eqref{eq:calc_vec_diff}.
%
%and \eqref{eq:ellipse_vec_diff}.
Substituting  the point of contact $\vec{x} = \vec{q}$ and simplifying results in
\begin{align}
\brak{\vec{V}\vec{q}+\vec{u}}\vec{m} & = 0 
\label{eq:ellipse_tangent_der_std}
\end{align}
%
which, upon taking the transpose, yields 
\eqref{eq:conic_tangent_mq}.
\end{enumerate}
