 Below is the solution :
\begin{align}
    \myvec{1 & 2 & 1}\myvec{1 & 2 & 0 \\2 & 0 & 1\\1 & 0 & 2}\myvec{0 \\ 2 \\ x}=0
\end{align}
\begin{multline}
    \implies \myvec{\myvec{1&2}&\myvec{1}}\myvec{\myvec{1&2\\2&0}&\myvec{0\\1}\\\myvec{1&0}&\myvec{2}}\myvec{\myvec{0\\2}\\\myvec{x}}=0
\end{multline}
    


\begin{multline}
\implies \myvec{\myvec{\myvec{1&2}\myvec{1&2\\2&0}\\+\\\myvec{1}\myvec{1&0}}&\myvec{\myvec{1&2}\myvec{0\\1}\\+\\\myvec{1}\myvec{2}}}\myvec{\myvec{0\\2}\\\myvec{x}}\\=0
\end{multline}

\begin{multline}
    \implies\myvec{\myvec{5&2}+\myvec{1&0}&\myvec{2+2}}\myvec{\myvec{0\\2}\\\myvec{x}}\\=0
\end{multline}
    
\begin{align}
    \implies \myvec{\myvec{6&2}&\myvec{4}}\myvec{\myvec{0\\2}\\\myvec{x}}=0
\\
    \implies \myvec{\myvec{6&2}\myvec{0\\2}+\myvec{4}\myvec{x}}=0
\\
    \implies \myvec{4+4\times x}=0
\\
    \implies 4\times x=-4
\\
    \implies x=-1
\end{align}
    




