%
\begin{enumerate}
\item From the given information,
\begin{align}
\norm{\vec{P}-\vec{A}}^2=\norm{\vec{P}-\vec{B}}^2
\\
\implies\norm{\vec{P}}^2+\norm{\vec{A}}^2-2\vec{A}^T\vec{P}
\\
=\norm{\vec{P}}^2+\norm{\vec{B}}^2-2\vec{B}^T\vec{P}
\\
\implies 2\vec{A}^T\vec{P}-2\vec{B}^T\vec{P}=\norm{\vec{A}}^2-\norm{\vec{B}}^2  \label{vec/29/eq1}
\end{align}
\item Equation of plane is $\vec{n}^T\vec{P}=\vec{d}$
\\
where,$\vec{n}^T$ is the normal vector to the plane 
\begin{itemize}
\item From \eqref{vec/29/eq1},
\begin{align}
\myvec{2\vec{A}^T-2\vec{B}^T}\vec{P}=\norm{\vec{A}}^2-\norm{\vec{B}}^2 \label{vec/29/eq2}
\end{align}
$\vec{P}$ is a plane and it is perpendicular bisector to $\vec{A}-\vec{B}$
\\
$\because\vec{P}$ is perpendicular to line joining $\vec{A}$ and $\vec{B}$
\item Midpoint of $\vec{A}$ and $\vec{B}$
\begin{align}
\vec{M}= \frac{\vec{A}+\vec{B}}{2}
\end{align}
\item Substitute in \eqref{vec/29/eq2},
\begin{align}
\myvec{2\vec{A}^T-2\vec{B}^T}\brak{\frac{\vec{A}+\vec{B}}{2}}
=\myvec{\vec{A}^T-\vec{B}^T}\myvec{\vec{A}+\vec{B}}
\\
=\vec{A}^T\vec{A}+\vec{A}^T\vec{B}-\vec{B}^T\vec{A}-\vec{B}^T\vec{B}
\end{align}
\begin{align}
\because \vec{A}^T\vec{A}=\norm{\vec{A}}^2,
\\
\vec{B}^T\vec{B}=\norm{\vec{B}}^2,
\\
\vec{A}^T\vec{B}=\vec{B}^T\vec{A}
\end{align}
\begin{align}
\implies\myvec{2\vec{A}^T-2\vec{B}^T}\brak{\frac{\vec{A}+\vec{B}}{2}}=\norm{\vec{A}}^2-\norm{\vec{B}}^2 
\end{align}
$\implies \frac{\vec{A}+\vec{B}}{2}$ satisfies \eqref{vec/29/eq1}
\item $\therefore$ $\vec{P}$ is the plane that is perpendicular bisector of the line joining the given points 
\end{itemize}
\item Putting given values $\vec{A}$ and $\vec{B}$ in \eqref{vec/29/eq1},we get 
\begin{align}
2\myvec{3 & 4 & -5}\vec{P}-2\myvec{-2 & 1 & 4}\vec{P}
\\
=\norm{\myvec{3\\4\\-5}}^2-\norm{\myvec{-2\\1\\4}}^2
\\
\implies\myvec{6 & 8 & -10}\vec{P}+\myvec{4 & -2 & -8}\vec{P} 
\\
=50-21
\\
\implies\myvec{10 & 6 & -18}\vec{P}=29
\end{align}
$\therefore$ The required equation is
\begin{align}
\myvec{10 & 6 & -18}\vec{P}=29
\end{align}
\end{enumerate}


