Given,
\\
\begin{align}
    F(x)=\myvec{
\cos{x} & -\sin{x} & 0\\
\sin{x} & \cos{x} & 0\\
0 & 0 & 1
}
\end{align}
Replacing x with y in above equation 2.0.1 F(y) is given as,
\begin{align}
    F(y)=\myvec{
\cos{y} & -\sin{y} & 0\\
\sin{y} & \cos{y} & 0\\
0 & 0 & 1
}
\end{align}
From the problem statement,\\
Consider the LHS,\\
F(x)F(y)
\begin{align}
&=\myvec{
\cos{x} & -\sin{x} & 0\\
\sin{x} & \cos{x} & 0\\
0 & 0 & 1
}\myvec{
\cos{y} & -\sin{y} & 0\\
\sin{y} & \cos{y} & 0\\
0 & 0 & 1
}\\
&=\myvec{
\cos{x}\cos{y}-\sin{x}\sin{y} & -\cos{x}\sin{y}-\sin{x}\cos{y} & 0\\
\sin{x}\cos{y}+\cos{x}\sin{y} & -\sin{x}\sin{y}+\cos{x}\cos{y} & 0\\
0 & 0 & 1
}\\
&=\myvec{
\cos{(x+y)} & -\sin{(x+y)} & 0\\
\sin{(x+y)} & \cos{(x+y)} & 0\\
0 & 0 & 1
}\\
&=F(x+y)
\end{align}
Therefore, 
\begin{align}
    F(x)F(y)=F(x+y)
\end{align}
