
Given
\begin{equation}
 A^2 = A \implies A^2 - A = 0 
\end{equation}
Let $\lambda $ is the eigen value then the every eigen value satisfies its very own characteristic equation
\begin{equation}\label{eq:solutions/matrix/77/eq1}
\implies  \lambda^2 = \lambda  \implies  \lambda^2 - \lambda = 0 
\end{equation}
Then $ (I+A)^3 - 7A $ can be written as $ (I+\lambda)^3 - 7\lambda $\\
\begin{align}
 (I+\lambda)^3 - 7\lambda &  = I^3+\lambda^3+3I^2\lambda+3\lambda^2I - 7\lambda
\end{align}
we know that 
\begin{align}	
I^3 = I^2 = 1
\end{align}
\begin{align}
   = 1+\lambda^3+3(1)\lambda+3\lambda^2(1)-7\lambda
\end{align}
\begin{align}
  = 1+\lambda^3+3\lambda+3\lambda^2-7\lambda
\end{align}
\begin{align}
    = 1+(\lambda^2\lambda)+3\lambda+3\lambda -7\lambda
\end{align}
\begin{align}
     = 1+(\lambda\lambda)-\lambda
\end{align}
\begin{align}
 = 1+\lambda^2-\lambda
\end{align}
From the equation \eqref{eq:solutions/matrix/77/eq1}  $ \lambda^2-\lambda = 0 $
\begin{align}
     = 1+0
\end{align}
\begin{align}
     = 1
\end{align}

Option C is the valid answer.


 


  
