\begin{align}
&\left(\frac{\vec{z_1z_2}}{\vec{z_1}^*}\right)=\myvec{2 & 1\\ -1 & 2}\myvec{-2 & -1\\ 1 & -2}\left[\myvec{2 & -1\\ 1 & 2}\right]^{-1}\myvec{1 \\0}\label{eq:solutions/complex/13eqn_4}\\
&\left(\frac{\vec{z_1z_2}}{\vec{z_1}^*}\right)=\myvec{2 & 1\\ -1 & 2}\myvec{-2 & -1\\ 1 & -2}\left[\frac{1}{5}\myvec{2 & 1\\ -1 & 2}\right]\myvec{1 \\0}\label{eq:solutions/complex/13eqn_5}\\
&\left(\frac{\vec{z_1z_2}}{\vec{z_1}^*}\right)=\frac{1}{5}\myvec{-2 & -11\\ 11 & -2}\myvec{1 \\0}\label{eq:solutions/complex/13eqn_6}\\
&\left(\frac{\vec{z_1z_2}}{\vec{z_1}^*}\right)=\frac{1}{5}\myvec{-2 \\11}\label{eq:solutions/complex/13eqn_7}
\end{align}
Hence, the real part of $\left(\frac{\vec{z_1z_2}}{\vec{z_1}^*}\right)=-\frac{2}{5}$

\begin{align}
&\left(\frac{1}{\vec{z_1}\vec{z_1}^*}\right)=(\vec{z_1}\vec{z_1}^*)^{-1}\label{eq:solutions/complex/13eqn_8}\\
&\left(\frac{1}{\vec{z_1}\vec{z_1}^*}\right)=\left[\myvec{2 & 1\\ -1 & 2}\myvec{2 & -1\\ 1 & 2}\right]^{-1}\myvec{1 \\0}\label{eq:solutions/complex/13eqn_9}\\
&\left(\frac{1}{\vec{z_1}\vec{z_1}^*}\right)=\left[\myvec{5 & 0\\ 0 & 5}\right]^{-1}\myvec{1 \\0}\label{eq:solutions/complex/13eqn_10}\\
&\left(\frac{1}{\vec{z_1}\vec{z_1}^*}\right)=\frac{1}{25}\myvec{5 & 0\\ 0 & 5}\myvec{1 \\0}\label{eq:solutions/complex/13eqn_11}\\
&\left(\frac{1}{\vec{z_1}\vec{z_1}^*}\right)=\frac{1}{25}\myvec{5 \\ 0}\label{eq:solutions/complex/13eqn_12}
\end{align}
Hence, the imaginary part of $\left(\frac{1}{\vec{z_1}\vec{z_1}^*}\right)=0$.
