\begin{align}
    \bm{d}=\bm{2a}-\bm{b}+\bm{3c}\\
    \bm{2a}=\begin{pmatrix}2\\2\\2\end{pmatrix}\\
    \bm{-b}=\begin{pmatrix}-2\\1\\-3\end{pmatrix}\\
    \bm{3c}=\begin{pmatrix}3\\-6\\3\end{pmatrix}
\end{align}
From the above, 
\begin{align}
    \bm{d}=\begin{pmatrix}3\\-3\\2\end{pmatrix}\\
    \norm{\bm{d}}=\sqrt{3^2+(-3)^2+2^2}=\sqrt{22}\\
    \bm{e}=\frac{\bm{d}}{\norm{\bm{d}}}
\end{align}
$\bm{e}$  is the unit vector parallel to given vector\\
Thus,
\begin{align}
    \boxed{\bm{e}=\frac{1}{\sqrt{22}}\begin{pmatrix}3\\-3\\2\end{pmatrix}}
\end{align}
