Given determinant:
\begin{align}
\Delta =\mydet{y+k&y&y\\y&y+k&y\\y&y&xy+k}
\end{align}
Applying transformation:
\begin{align}
\xleftrightarrow[]{R_1 \leftarrow R_1+ R_2+ R_3} 
\mydet{3y+k&3y+k&3y+k\\y&y+k&y\\y&y&y+k}
\\
\xleftrightarrow[]{C_2 \leftarrow C_2- C_1} 
\mydet{3y+k&0&3y+k\\y&k&y\\y&0&y+k}
\\
\xleftrightarrow[]{C_3 \leftarrow C_3- C_1} 
\mydet{3y+k&0&0\\y&k&0\\y&0&k}
\end{align}
Taking determinant
\begin{align}
\implies\Delta =(3y+k)k^2\\
\mydet{y+k&y&y\\y&y+k&y\\y&y&xy+k}=k^2(3y+k)
\end{align}
Hence proved.
