Let,
\begin{align}
 \vec P &=\vec{X};
\end{align}
 so,
 \begin{align}
 \vec{(PA)}^2&=\norm{\vec P-\vec A}^2\\
 &=\norm{\vec X-\vec A}^2\\
 &=\norm{\vec X}^2+\norm{\vec A}^2-2\vec X^T\vec A\label{vec/25/eq1}
 \end{align}
 and
 \begin{align}
 \vec{(PB)}^2&=\norm{\vec P-\vec B}^2\\
 &=\norm{\vec X-\vec B}^2\\
 &=\norm{\vec X}^2+\norm{\vec B}^2-2\vec X^T\vec B\label{vec/25/eq2}
 \end{align}
 The given equation is
\begin{align}
 \vec{(PA)}^2+ \vec{(PB)}^2 =2k^2\label{vec/25/eq3}
 \end{align}
 Sub \eqref{vec/25/eq1} and \eqref{vec/25/eq2}   values in \eqref{vec/25/eq3} 
\begin{align}
\norm{\vec X}^2+\norm{\vec A}^2-2\vec X^T\vec A+\norm{\vec X}^2+\norm{\vec B}^2-2\vec X^T\vec B=2k^2\\
\implies 2\norm{\vec X}^2+\norm{\vec A}^2+\norm{\vec B}^2-2\vec X^T(\vec A+\vec B)=2k^2\label{vec/25/eq4} 
\end{align}
sub $\vec A$,$\vec B$ values in equation \eqref{vec/25/eq4} ,we get
\begin{align}
 2\norm{\vec X}^2+\norm{\myvec{3\\4\\5}}^2+\norm{\myvec{-1\\3\\-7}}^2-2\vec X^T\brak{\myvec{3\\4\\5}+\myvec{-1\\3\\-7}}=2k^2
 \end{align}
 $\therefore$ the required equation is
 \begin{align}
  2\norm{\vec X}^2-2\vec X^T\myvec{2\\7\\-2}+109-2k^2=0
\end{align}