Let $\vec{A}=\vec{a}+\vec{b} \ and\  \vec{B}=\vec{a}-\vec{b}$
\begin{align}
\vec{A} = \myvec{3\\2\\2\\} + \myvec{1\\2\\-2\\} = \myvec{4\\4\\0\\}
\end{align}
\begin{align}
\vec{B} = \myvec{3\\2\\2\\} - \myvec{1\\2\\-2\\}=\myvec{2\\0\\4\\}
\end{align}
Let $\vec{n}$ be a vector Perpendicular to $\vec{A}$ and $\vec{B}$ both
	\begin{align}
		\vec{A}^{T}\vec{n} &= 0 \\
		\vec{B}^{T}\vec{n} &= 0
	\end{align} 
The augmented matrix can be represented as follows:
    \begin{align}
		\myvec{
			4 & 4 & 0 & \vrule & 0 \\
			2 & 0 & 4 & \vrule & 0 \\
		}
	\end{align}
	Using row reduction to find an expression for $\vec{n}$.
	    \begin{align}
		\xleftrightarrow[R_2 \leftarrow R_2-2R_1]{R_1 \leftarrow \frac{R_1}{4}}
		\myvec{
			1 & 1 & 0 & \vrule & 0 \\
			0 & -2 & 4 & \vrule & 0 \\
		}
		\\
		\xleftrightarrow[R_1 \leftarrow R_1-R_2]{R_2 \leftarrow \frac{R_2}{-2}}
		\myvec{
			1 & 0 & 2 & \vrule & 0 \\[0.2cm]
			0 & 1 & -2 & \vrule & 0 \\[0.2cm]
		}
	\end{align}
From above equations we get,
  \begin{align}
\therefore \myvec{n_1\\n_2\\n_3} = \myvec{-2n_3\\2n_3\\n_3} = n_3\myvec{-2\\2\\1}
  \end{align}
Let us consider $n_{3}$ to be 1 which gives us:
\begin{align}
\therefore \vec{n} = \myvec{-2\\2\\1\\}
\end{align}
\begin{align}      
\norm{{\vec{n}}}=\sqrt{(-2)^2+2^2+1^2}=3
\end{align}
Let $\vec{u}$ be the unit vector of $\vec{n}$ which can be found as follows:
\begin{align}      
\vec{u}=\frac{{\vec{n}}}{\norm{{\vec{n}}}}
\end{align}
Solving the above equation gives the unit vector $\vec{u}$ which is perpendicular to vectors $\vec{A} \ and \ \vec{B}$
\begin{align}
\boxed{\therefore \vec{u} = \frac{1}{3} \myvec{2\\-2\\-1\\}}
\end{align}

