\begin{align}
LHS=\begin{vmatrix}
x&x^2&1+px^3\\y&y^2&1+py^3\\z&z^2&1+pz^3
\end{vmatrix}
\end{align}
By expanding using sum property
\begin{align}
=\begin{vmatrix}
x&x^2&1\\y&y^2&1\\z&z^2&1
\end{vmatrix}
+\begin{vmatrix}
x&x^2&px^3\\y&y^2&py^3\\z&z^2&pz^3
\end{vmatrix}
\end{align}
By using switching of rows(or columns) property
\begin{align}
=(-1)\begin{vmatrix}
1&x^2&x\\1&y^2&y\\1&z^2&z
\end{vmatrix}
+\begin{vmatrix}
x&x^2&px^3\\y&y^2&py^3\\z&z^2&pz^3
\end{vmatrix}\\
=(-1)^2\begin{vmatrix}
1&x&x^2\\1&y&y^2\\1&z&z^2
\end{vmatrix}
+\begin{vmatrix}
x&x^2&px^3\\y&y^2&py^3\\z&z^2&pz^3
\end{vmatrix}
\end{align}
By using scalar multiplication property
\begin{align}
=\begin{vmatrix}
1&x&x^2\\1&y&y^2\\1&z&z^2
\end{vmatrix}
+(pxyz)\begin{vmatrix}
1&x&x^2\\1&y&y^2\\1&z&z^2
\end{vmatrix}\\
=(1+pxyz)\begin{vmatrix}
1&x&x^2\\1&y&y^2\\1&z&z^2
\end{vmatrix}
\end{align}
By applying row reduction
\begin{align}
=(1+pxyz)\begin{vmatrix}
1&x&x^2\\1&y&y^2\\1&z&z^2
\end{vmatrix}\\
 \xleftrightarrow[]{R_2 \leftarrow R_2-R_3}
(1+pxyz)\begin{vmatrix}
1&x&x^2\\0&y-z&y^2-z^2\\1&z&z^2
\end{vmatrix}\\
 \xleftrightarrow[]{R_3 \leftarrow R_3-R_1}
(1+pxyz)\begin{vmatrix}
1&x&x^2\\0&y-z&y^2-z^2\\0&z-x&z^2-x^2
\end{vmatrix}
\end{align}
By using scalar multiplication property
\begin{align}
=(1+pxyz)(y-z)(z-x)\begin{vmatrix}
1&x&x^2\\0&1&y+z\\0&1&z+x
\end{vmatrix}
\end{align}
By applying the determinant formula
\begin{align}
=(1+pxyz)(y-z)(z-x)(z+x-y-z)\\
=(1+pxyz)(x-y)(y-z)(z-x)\\
= RHS
\end{align}
Hence Proved.
