
Multiplying above equation with $\vec{A}^{-1}$ on both sides, We get :
\begin{align}
\implies \vec{A}^2\vec{A}^{-1} - 5\vec{A}\vec{A}^{-1} + 7\vec{I}\vec{A}^{-1} &= 0 \\
\implies \vec{A}\vec{A}\vec{A}^{-1} - 5\vec{I} + 7\vec{A}^{-1} &= 0 \\
\implies \vec{A}\vec{I} - 5\vec{I} + 7\vec{A}^{-1} &= 0\\
\implies \vec{A}^{-1} &= \frac{1}{7}\brak{5\vec{I} - \vec{A}}
\end{align}

Solving for $\vec{A}^{-1}$, we get :
\begin{align}
    \vec{A}^{-1} &= \frac{1}{7}\brak{5\myvec{ 1 & 0\\ 0 & 1} - \myvec{ 3 & 1\\ -1 & 2}} \\
    \implies \vec{A}^{-1} &= \frac{1}{7}\brak{\myvec{ 2 & -1\\ 1 & 3}}
\end{align}

