Let 
\begin{align}
\vec{a}=\myvec{
1\\
-2\\
3
}
\vec{b} = \myvec{
3\\
-2\\
1
}
\end{align}
Angle between the vectors is given by,
\begin{align}
    \theta      &=\cos^{-1}\left(\frac{\vec{a}^T\vec{b}}{\norm{\vec{a}}\norm{\vec{b}}}\right)\\
    \norm{\vec{a}}&=\sqrt{1^2+(-2)^2+3^2}=\sqrt{14} \\
    \norm{\vec{b}}&=\sqrt{3^2+(-2)^2+1^2}=\sqrt{14}\\
    \vec{a}^T\vec{b}&=(1)(3)+(-2)(-2)+(3)(1)=10\\
    \theta&=\cos^{-1}\left(\frac{10}{(\sqrt{14})(\sqrt{14)}}\right)\\
    &=\cos^{-1}\left(\frac{10}{14}\right)\\
\end{align}

