
The given polynomial can be expressed as:
\begin{align}
\vec{x}^T \myvec{6 & 0\\0 & 0}\vec{x}+ \myvec{17 & 0}\vec{x}+5=0
\end{align}
Substituting y=0 in the above equation,
\begin{align}
 6x^2+17x+5 &=0\\
\implies x&=\frac{-1}3{},\frac{-5}{2}\\
\therefore (3x+1)(2x+5) &=6x^2+17x+5
\end{align}
%
which is verified in Fig.     \ref{quadform/16/Fig:Graph Of $x^2+7x+10 &=$.}

\begin{figure}[ht!]
    \centering
    \includegraphics[width=\columnwidth]{solutions/su2021/2/16/Graph.png}
    \caption{Graph of $6x^2+17x+5$.}
    \label{quadform/16/Fig:Graph Of $x^2+7x+10 &=$.}
\end{figure}


