In our case, 

\begin{align}
\myvec{1\\1}= \myvec{1 & -1\\1 & 1}\myvec{1\\0}
\end{align}

\begin{align}
\myvec{1\\-1}= \myvec{1 & 1\\-1 & 1}\myvec{1\\0}
\end{align}

Now,

\begin{align}
     \frac{\myvec{1\\1}}{\myvec{1\\-1}}= \myvec{1 & -1\\1 & 1}\myvec{1 & 1\\-1 & 1}^{-1}\myvec{1\\0}\\
      = \myvec{0\\1}
\end{align}

Similarly,

\begin{align}
     \frac{\myvec{1\\-1}}{\myvec{1\\1}} = \myvec{1 & 1\\-1 & 1}\myvec{1 & -1\\1 & 1}^{-1}\myvec{1\\0}\\
      = \myvec{0\\-1}
\end{align}

So,

\begin{align}
\frac{\myvec{1\\1}}{\myvec{1\\-1}} - \frac{\myvec{1\\-1}}{\myvec{1\\1}} = \myvec{0\\1} - \myvec{0\\-1} \\
      = \myvec{0\\2}
\end{align}
Now, according to the problem statement:
\begin{align}
\frac{\myvec{1\\1}}{\myvec{1\\-1}} - \frac{\myvec{1\\-1}}{\myvec{1\\1}} \\
      = \myvec{0\\2}
\end{align} 
$\therefore$ 
\begin{align}
\norm{\frac{\myvec{1\\1}}{\myvec{1\\-1}} - \frac{\myvec{1\\-1}}{\myvec{1\\1}}} \\
      =\norm{\myvec{0\\2}} = \sqrt{0^2 + 2^2} = 2
\end{align} 
So, we can say that the modulus value of 
\begin{align}
\frac{\myvec{1\\1}}{\myvec{1\\-1}} - \frac{\myvec{1\\-1}}{\myvec{1\\1}}
\end{align} is 2.

