
The given equation of line is,
\begin{equation}\label{eq:solutions/line_plane/44/eq1}
		\vec{n}^T\vec{x} = c
\end{equation}

where $ \vec{n} = \myvec{\sqrt{3}&1}$ and $c = -2 $
		\\
Now obtain a new equation,
\begin{equation}
\frac{\vec{n}}{\norm{\vec{n}}}\vec{x}= \frac{c}{\norm{\vec{n}}};
\end{equation}

where $ \norm{\vec{n}}$ is the norm of the $\vec{n}\implies $

 \begin{equation}\label{eq:solutions/line_plane/44/eq:subeq3}
   \vec{u}^T\vec{x} = P
\end{equation}

where $\vec{u} = \myvec{\cos \theta  \\   \sin \theta}$ and $ P = \frac{c}{\norm{\vec{n}}}$

Substituting the values of $\vec{n}$ and c, we get
\begin{equation}\label{eq:solutions/line_plane/44/eq:subeq4}
		\norm{\vec{n}} = 2
\end{equation}
\begin{equation}\label{eq:solutions/line_plane/44/eq:subeq5}
		\myvec{\sqrt{3}/2 & 1/2}\vec{x} = -1
\end{equation}
\begin{equation}\label{eq:solutions/line_plane/44/eq:subeq6}
		\myvec{-\sqrt{3}/2& -1/2}\vec{x} = 1		
\end{equation}	
From \eqref{solutions/line_plane/44/eq:subeq3} and \eqref{solutions/line_plane/44/eq:subeq6}. we derive,
\begin{equation}
		\cos\theta = -\sqrt{3}/2\ ;\hspace{3mm} \sin\theta = -1/2
\end{equation}
\begin{equation}
		 P = 1
\end{equation}
%\begin{equation}
%		\therefore\ \hspace{1mm} \theta = \cos^{-1}(\frac{-\sqrt{3}}{2}) = \sin^{-1}(\frac{-1}{2}) = \ang{210}\hspace{3mm},\hspace{3mm} P = 1
%	\end{equation}
