
Equation \ref{eq:solutions/chem/7b1}  can be written as :

\begin{align}
\label{eq:solutions/chem/7b2} Zn+ AgNO_{3} \to Ag + Zn(NO_{3})_{2}
\end{align}

Suppose balance form of the equation is :
\begin{align}
    \label{eq:solutions/chem/7b3} x_{1}Zn+ x_{2}AgNO_{3} \to x_{3}Ag + x_{4} Zn(NO_{3})_{2}
\end{align}
which results in the following equations:
\begin{align}
    ( x_{1} - 2x_{4} ) Zn = 0\\
    ( x_{2} - x_{3} ) Ag = 0\\
    ( x_{3} - 2 x_{4} ) N =0\\
    ( 3x_{3} - 6x_{4} ) O = 0
\end{align}
which can be expressed as
\begin{align}
    x_{1} + 0.x_{2} + 0.x_{3} - x_{4} = 0\\
    0.x_{1} + x_{2} - x_{3} + 0.x_{4} = 0\\
    0.x_{1} + 0.x_{2} + x_{3} - 2.x_{4} =0\\
    0.x_{1} + 0.x_{2} + 3x_{3} - 6.x_{4}= 0
\end{align}
resulting in the matrix equation
\begin{align}
    \label{eq:solutions/chem/7b: matrix}
    \myvec{1 & 0 & 0 & -1\\
           0 & 1 & -1 & 0\\
           0 & 0 & 1 & -2\\
           0 & 0 & 3 & -6 }\vec{x}
           =\vec{0}
\end{align}
where,
\begin{align}
   \vec{x}= \myvec{x_{1}\\x_{2}\\x_{3}\\x_{4}}
\end{align}
(\ref{eq:solutions/chem/7b: matrix}) can be reduced as follows:
\begin{align}
    \myvec{1 & 0 & 0 & -1\\
   	0 & 1 & -1 & 0\\
   	0 & 0 & 1 & -2\\
   	0 & 0 & 3 & -6 }
    \xleftrightarrow {R_{4}\leftarrow R_4 - 3R_3}
      \myvec{1 & 0 & 0 & -1\\
    	0 & 1 & -1 & 0\\
    	0 & 0 & 1 & -2\\
    	0 & 0 & 0 & 0 }
    \end{align}
Thus,
\begin{align}
    x_1 = x_4, x_ 2 = 2x_4, x_3 = 2x_4\\
    \implies \quad\vec{x } = \myvec{x_{4} \\ 2x_{4}\\ 2x_{4} \\ x_{4}}   =  x_4 \myvec{1\\ 2 \\ 2 \\1}
    \end{align} 
by substituting $x_4= 1$, we get :
\begin{align}
 \implies \quad\vec{x} = \myvec{1\\ 2 \\ 2 \\1}
\end{align}

%\vspace{5mm} 
Hence, (\ref{eq:solutions/chem/7b3}) finally becomes
\begin{align}
Zn + 2AgNO_{3} \to 2Ag + Zn(NO_{3})_{2}
\end{align}
