Given that $\vec{A}$ =$\myvec{1&2&3\\3&-2&1\\4&2&1}$.
\begin{enumerate}
\item \textbf{The Characteristic equation} is given by:
\begin{align}
  \implies  \abs{\vec{A}-\lambda\vec{I}}&=0
    \\
    \implies \mydet{1-\lambda&2&3\\3&-2-\lambda&1\\4&2&1-\lambda}&=0
    \end{align}
\begin{multline}
   \implies\brak{1-\lambda}\brak{\brak{-2-\lambda}\brak{1-\lambda}-2}
   \\
   -2\brak{3\brak{1-\lambda}-4}+3\brak{6+4\brak{2+\lambda}}=0
\end{multline}
\begin{align}
 \implies   \lambda^3-23\lambda-40=0
\end{align}
The above equation is similar to equation to be proved.
\item According to \textbf{Cayley-Hamilton Theorem:} 
\\
Every square matrix satisfies its own
\\\textbf{characteristic equation}.
\begin{align}
\therefore    \vec{A}^3-23\vec{A}-40\vec{I}=0
\end{align}
Hence Proved.
\end{enumerate}