
Given 
\begin{equation}
\vec{B} = 
\begin{pmatrix} 
2 & -2 & -4 \\  -1 & 3 & 4 \\ 1&-2&-3
\end{pmatrix}
\end{equation}
and \begin{equation}
\vec{B^\top} = 
\begin{pmatrix} 
2 & -1 & 1 \\ -2 & 3 & -2 \\ -4 & 4 & -3
\end{pmatrix} 
\end{equation} 
\begin{align}
  \vec{C} &= \frac{\vec{B}+\vec{B^\top}}{2} = \begin{pmatrix} 
2 & -\frac{3}{2} & -\frac{3}{2} \\  -\frac{3}{2} & 3 & 1 \\ -\frac{3}{2}&1&-3
\end{pmatrix}
\\
&=\vec{C^\top}
\label{eq1}
\end{align}
Also,

\begin{align}
\vec{D} &=\frac{\vec{B} - \vec{B^\top}}{2} =
\begin{pmatrix} 
0 & -\frac{1}{2} & -\frac{5}{2} \\  \frac{1}{2} & 0 & 3 \\ \frac{5}{2}&-3&0
\end{pmatrix}\\
&= -\vec{D^\top}
\label{eq2}
\end{align}
Hence, $\vec{C}$ is a symmetric matrix and $\vec{D}$ is skew symmetric.
and $\vec{C} + \vec{D}$ = $\vec{B}$.

