\begin{enumerate}
    \item \begin{align} 
   \Vec{A}=&\myvec{5\\ \dfrac{1}{2}\\-1}
    \end{align}
   
          transpose of $\Vec{A}$ is given as $\Vec{A}^{\top}$
    
    \begin{align} 
         (\Vec{A}^{\top})_{i j} =& \Vec{A}_{j i}\\
          \therefore \Vec{A}^{\top} = &\myvec{5& \dfrac{1}{2}&-1}
    \end{align}
    \item \begin{align} 
    \Vec{B}=&\myvec{1&-1\\2&3}
    \end{align}
  
          transpose of $\Vec{B}$ is given as $\Vec{B}^{\top}$
    
    \begin{align}
         (\Vec{B}^{\top})_{i j} =& \Vec{B}_{j i}\\
          \therefore \Vec{B}^{\top} = &\myvec{1&2\\-1&3}
    \end{align}
    \item \begin{align} 
    \Vec{C}=&\myvec{-1&5&6\\ \sqrt{3}&5&6\\2&3&-1}
    \end{align}
   
          transpose of $\Vec{C}$ is given as $\Vec{C}^{\top}$
    
    \begin{align}
         (\Vec{C}^{\top})_{i j} =& \Vec{C}_{j i}\\
          \therefore \Vec{C}^{\top} = &\myvec{-1& \sqrt{3}&2\\ 5&5&3\\6&6&-1}
    \end{align}
\end{enumerate}