
 \begin{align}
  \mydet{x&\sin\theta&\cos\theta\\-\sin\theta&-x&1\\\cos\theta&1&x}
  \end{align}
  Now, Solving the determinant:-
  

  \begin{multline}
  =x(-x^{2}-1)-\sin\theta(-x\sin\theta-\cos\theta)\\
  +\cos\theta(-\sin\theta+x\cos\theta)
  \\
  =-x^{3}-x+x\sin^{2}\theta+\sin\theta\cos\theta \\ 
  -\sin\theta\cos\theta+x\cos^{2}\theta\\
  \end{multline}
 \begin{align}
  =-x^{3}-x+x\sin^{2}\theta+x\cos^{2}\theta\\
  =-x^{3}(\because \sin^{2}\theta+\cos^{2}\theta=1)
  \end{align}
  Hence, the determinant is independent of $\theta$.
