\begin{enumerate}
    \item Below is the solution :
\begin{align}
    \cfrac{\myvec{1 \\ 7}}{\myvec{2 \\ -1}^{2}}
\\
    \myvec{2 \\ -1}^2 = \myvec{2 & 1\\-1 & 2}\myvec{2 & 1\\-1 & 2}\myvec{1 \\ 0}
\\
    \implies \myvec{2 \\ -1}^2 = \myvec{3 & 4\\-4 & 3}\myvec{1 \\ 0}
\\
    \implies \myvec{2 \\ -1}^2 = \myvec{3 \\-4}
\\
    =\myvec{1 \\ 7}\myvec{3\\-4}^{-1}
\\
    =\cfrac{1}{25}\myvec{1 & -7\\7 & 1}\myvec{3 & -4\\4 & 3}\myvec{1 \\ 0}
\\
    =\cfrac{1}{25}\myvec{-25 & -25\\25 & -25}\myvec{1 \\ 0}
\\
    =\cfrac{25}{25}\myvec{-1 & -1\\1 & -1}\myvec{1 \\ 0}
\\
    =\sqrt{2}\myvec{\cfrac{-1}{\sqrt{2}} & \cfrac{-1}{\sqrt{2}} \\ \cfrac{1}{\sqrt{2}} & \cfrac{-1}{\sqrt{2}}}
\\
    =\sqrt{2}\myvec{\cos{135}\degree & -\sin{135}\degree\\ \sin{135}\degree & \cos{135}\degree}\myvec{1 \\ 0}
\\
    =\sqrt{2}\myvec{\cos{135}\degree \\ \sin{135}\degree}
\\
    =\sqrt{2} \angle 135 \degree
\end{align}
\item Below is the solution:
\begin{align}
    \cfrac{\myvec{1 \\ 3}}{\myvec{1 \\ -2}}
\\
    \myvec{1 \\ -2} = \myvec{1 & 2\\-2 & 1}\myvec{1 \\ 0}
\\
    =\myvec{1 \\ 7}\myvec{1\\-2}^{-1}
\\
    =\cfrac{1}{5}\myvec{1 & -3\\3 & 1}\myvec{1 & -2\\2 & 1}\myvec{1 \\ 0}
\\
    =\cfrac{1}{5}\myvec{-5 & -5\\5 & -5}\myvec{1 \\ 0}
\\
    =\cfrac{5}{5}\myvec{-1 & -1\\1 & -1}\myvec{1 \\ 0}
\\
    =\sqrt{2}\myvec{\cfrac{-1}{\sqrt{2}} & \cfrac{-1}{\sqrt{2}} \\ \cfrac{1}{\sqrt{2}} & \cfrac{-1}{\sqrt{2}}}
\\
    =\sqrt{2}\myvec{\cos{135}\degree & -\sin{135}\degree\\ \sin{135}\degree & \cos{135}\degree}\myvec{1 \\ 0}
\\
    =\sqrt{2}\myvec{\cos{135}\degree \\ \sin{135}\degree}
\\
    =\sqrt{2} \angle 135 \degree
\end{align}
\end{enumerate}


