The points are obtained by substituting
\begin{align}
\vec{x} &= \myvec{a\\0},
\vec{x} &=\myvec{0\\b},
\vec{x} &= \myvec{c\\1},
\vec{x} &= \myvec{1\\d}
\end{align}
\begin{enumerate}
%
\item 
\begin{enumerate}
\begin{align}
\myvec{2&1}\myvec{a\\0} &= 7 \\
\implies a&=\frac{7}{2}
\end{align}
\item 
%
\begin{align}
\myvec{2&1}\myvec{0\\b} &= 7 \\
\implies b&=7
\end{align}
\item 
\begin{align}
\myvec{2&1}\myvec{c\\1} &= 7 \\
\implies c&=3  
\end{align}
\item
\begin{align}
\myvec{2&1}\myvec{1\\d} &= 7 \\
\implies d&=5 
\end{align}
\end{enumerate}
\item 
\begin{enumerate}
\item 
\begin{align}
\myvec{\pi&1}\myvec{a\\0} &= 9 \\
\implies a&=\frac{9}{\pi} 
\end{align}

\item 
\begin{align}
\myvec{\pi&1}\myvec{0\\b} &= 9 \\
\implies b&=9
\end{align}

\item 
\begin{align}
\myvec{\pi&1}\myvec{c\\1} &= 9 \\
\implies c&=\frac{8}{\pi}  
\end{align}

\item 
\begin{align}
\myvec{\pi&1}\myvec{1\\d} &= 9 \\
\implies d&=9-\pi
\end{align}
\end{enumerate}
\item 
\begin{enumerate}
 \item 
\begin{align}
\myvec{1&-4}\myvec{a\\0} &= 0 \\
\implies a&=0 
\end{align}

\item  
\begin{align}
\myvec{1&-4}\myvec{0\\b} &= 0 \\
\implies b&=0
\end{align}

\item  
\begin{align}
\myvec{1&-4}\myvec{c\\1} &= 0 \\
\implies c&=4  
\end{align}

\item  
\begin{align}
\myvec{1&-4}\myvec{1\\d} &= 0 \\
\implies d&=\frac{1}{4}
\end{align}

\end{enumerate}

\end{enumerate}
